Std/Classes/Order.lean
@@ -82,6 +82,9 @@ theorem cmp_congr_left (xy : cmp x y = .eq) : cmp x z = cmp y z :=
     | .gt => nomatch le_trans (nomatch ·.symm.trans xy) (nomatch ·.symm.trans yz) xz
     | .eq => rfl
 
+theorem cmp_congr_left' (xy : cmp x y = .eq) : cmp x = cmp y :=
+  funext fun _ => cmp_congr_left xy
+
 theorem cmp_congr_right [TransCmp cmp] (yz : cmp y z = .eq) : cmp x y = cmp x z := by
   rw [← Ordering.swap_inj, symm, symm, cmp_congr_left yz]
 
